examples/store_sess/proofs/client/store.v
@@ -45,29 +45,29 @@ Lemma wp_client_store skI skR cs t1 t2 t2' :
   {{{ RET #(); db_connected skI skR cs ∗ db_mapsto skI skR t1 t2' }}}.
 Proof.
 iIntros "#? #ctx #p_t1 #p_t2 !> %Φ [client mapsto] post".
-iDestruct "client" as "(%db & conn & rel & ready & state)".
+iDestruct "client" as "(%odb & %db & conn & rel & token & state)".
 iMod (DB.db_state_update t2' with "state mapsto") as "[state mapsto]".
 wp_lam. wp_pures. wp_list. wp_term_of_list.
 wp_bind (tag _ _). iApply wp_tag.
 wp_bind (Sess.send _ _).
 iApply (wp_send_msg _ _ _ _
-          (iMsg_tag (db_arms skI skR cs (db_st skI skR cs) db)) _
-          (db_st skI skR cs (<[t1 := t2']> db))
-          with "[conn]").
+          (iMsg_tag (db_arms skI skR cs (db_st skI skR cs) odb)) _
+          (db_st skI skR cs (Some (<[t1 := t2']> db)))
+          with "[conn token]").
 { iSplitL "conn".
   { iApply (connected_le with "conn"). iNext.
     iApply iProto_le_of_equiv. exact: db_st_unfold. }
   iSplitR.
   { rewrite public_tag public_of_list /=. by iFrame "#". }
+  iDestruct "token" as "[#?|token]"; eauto.
   iRight.
   iApply (iMsg_tag_intro _ _ (db_arms_store _ _ _ _ _)).
-  rewrite iMsg_exist_eq /=. iExists t1. iExists t2'.
+  rewrite iMsg_exist_eq /=. iExists db, t1, t2'.
   rewrite iMsg_base_eq /=.
-  do 2 (iSplit; first done).
-  auto. }
+  by do !iSplit. }
 iIntros "!> conn". wp_pures.
 iApply "post". iFrame "mapsto". iModIntro.
-iExists (<[t1 := t2']> db). iFrame.
+iExists (Some (<[t1 := t2']> db)), _. iFrame. by iRight.
 Qed.
 
 End Verif.
