examples/store_sess/proofs/server.v
@@ -54,30 +54,33 @@ Lemma wp_server_handle_store skI skR cs vdb :
 Proof.
 iIntros "#? #ctx".
 rewrite /server_handler /=.
-iIntros "!> %db %t %p !> %Φ (conn & rel & (#p_db & vdb & slot) & #p_t & disj) post".
+iIntros "!> %odb %db %t %p".
+iIntros "!> %Φ (conn & rel & (#p_db & vdb & token) & #p_t & disj) post".
 rewrite lookup_fmap db_arms_store /=.
 wp_pures. rewrite /Server.handle_store. wp_pures.
-iDestruct "disj" as "[#pub|car]".
--
-  wp_list_of_term t; wp_pures; last first.
-  { iApply ("post" $! true). iModIntro. iExists db. iFrame "rel vdb slot p_db".
+iPoseProof (or_sep1 with "token disj") as "token".
+iDestruct "token" as "[#pub|[token car]]".
+- wp_list_of_term t; wp_pures; last first.
+  { iApply ("post" $! true). iModIntro. iExists odb, db.
+    iFrame "rel vdb p_db". iSplitL; eauto.
     by iApply (connected_repoint with "conn pub"). }
   wp_list_match => [k v ->|_]; wp_pures; last first.
-  { iApply ("post" $! true). iModIntro. iExists db. iFrame "rel vdb slot p_db".
+  { iApply ("post" $! true). iModIntro. iExists odb, db.
+    iFrame "rel vdb p_db". iSplitL; eauto.
     by iApply (connected_repoint with "conn pub"). }
   rewrite public_of_list /=. iDestruct "p_t" as "(p_k & p_v & _)".
   wp_bind (AList.insert _ _ _).
   iApply (AList.wp_insert with "vdb").
   iIntros "!> vdb". rewrite -fmap_insert. wp_pures.
-  iApply ("post" $! true). iModIntro. iExists (<[k := v]> db).
-  iFrame "rel vdb slot".
-  iSplitL "conn"; first by iApply (connected_repoint with "conn pub").
+  iApply ("post" $! true). iModIntro. iExists (Some (<[k := v]> db)), _.
+  iFrame "rel vdb".
+  iSplitL; first by iApply (connected_repoint with "conn pub").
+  iSplitL; eauto.
   by iApply public_db_insert.
--
-  iDestruct "car" as (p1) "[car #HeqD]".
-  rewrite iMsg_exist_eq /=. iDestruct "car" as (k) "car".
-  iDestruct "car" as (v) "car".
-  rewrite iMsg_base_eq /=. iDestruct "car" as "(%e_t & #Heq1 & _)".
+- iDestruct "car" as (p1) "[car #HeqD]".
+  rewrite iMsg_exist_eq /=.
+  iDestruct "car" as (db' k v) "car".
+  rewrite iMsg_base_eq /=. iDestruct "car" as "(%e_t & #Heq1 & token')".
   subst t.
   rewrite !later_equivI_1.
   rewrite public_of_list /=. iDestruct "p_t" as "(p_k & p_v & _)".
@@ -89,12 +92,14 @@ iDestruct "disj" as "[#pub|car]".
   wp_bind (AList.insert _ _ _).
   iApply (AList.wp_insert with "vdb").
   iIntros "!> vdb". rewrite -fmap_insert. wp_pures.
-  iApply ("post" $! true). iModIntro. iExists (<[k := v]> db).
-  iFrame "rel vdb slot".
+  iApply ("post" $! true).
+  iExists (Some (<[k := v]> db)), _.
+  iFrame "rel vdb".
+  iMod (db_update_token (<[k := v]> db) with "token' token") as "(<- & token)".
   iSplitL "conn".
-  { iApply (connected_le with "conn"). iNext.
+  { iApply (connected_le with "conn"). iModIntro. iNext.
     iRewrite "HeqD". iRewrite -"Heq1". iApply iProto_le_refl. }
-  by iApply public_db_insert.
+  iModIntro. iFrame. by iApply public_db_insert.
 Qed.
 
 Lemma wp_server_handle_load skI skR cs vdb :
@@ -110,31 +115,33 @@ Lemma wp_server_handle_load skI skR cs vdb :
 Proof.
 iIntros "#? #ctx".
 rewrite /server_handler /=.
-iIntros "!> %db %t %p !> %Φ (conn & rel & (#p_db & vdb & slot) & #p_t & disj) post".
+iIntros "!> %odb %db %t %p".
+iIntros "!> %Φ (conn & rel & (#p_db & vdb & token) & #p_t & disj) post".
 rewrite lookup_fmap db_arms_load /=.
 wp_pures. rewrite /Server.handle_load. wp_pures.
-iDestruct "disj" as "[#pub|car]".
--
-  wp_bind (AList.find _ _).
+iPoseProof (or_sep1 with "token disj") as "disj".
+iDestruct "disj" as "[#pub|[token disj]]".
+- wp_bind (AList.find _ _).
   iApply (AList.wp_find with "vdb").
   iIntros "!> vdb". rewrite lookup_fmap.
   case e: (db !! t) => [v0|] /=; wp_pures; last first.
-  { iApply ("post" $! true). iModIntro. iExists db. iFrame "rel vdb slot p_db".
+  { iApply ("post" $! true). iModIntro. iExists (Some db), db.
+    iFrame "rel vdb p_db". iSplitL; eauto.
     by iApply (connected_repoint with "conn pub"). }
   iPoseProof (big_sepM_lookup _ _ _ _ e with "p_db") as "[_ p_v0]".
   wp_bind (Sess.send _ _).
-  iApply (wp_send _ _ _ _ v0 (iProto_dual (db_st skI skR cs db))
+  iApply (wp_send _ _ _ _ v0 (iProto_dual (db_st skI skR cs (Some db)))
            with "[conn]").
   { iSplit => //.
     by iApply (connected_repoint with "conn pub"). }
   iIntros "!> conn". wp_pures.
-  iApply ("post" $! true). iModIntro. iExists db.
-  by iFrame "rel vdb slot p_db conn".
--
-  iDestruct "car" as (p1) "[car #HeqD]".
-  rewrite iMsg_exist_eq /=. iDestruct "car" as (k1) "car".
-  rewrite iMsg_base_eq /=. iDestruct "car" as "(%e_t & #Heq1 & %HkS)".
+  iApply ("post" $! true). iModIntro. iExists (Some db), db.
+  by iFrame "rel vdb p_db conn"; eauto.
+- iDestruct "disj" as (p1) "[car #HeqD]".
+  rewrite iMsg_exist_eq /=. iDestruct "car" as (db0 k1) "car".
+  rewrite iMsg_base_eq /=. iDestruct "car" as "(%e_t & #Heq1 & token' & %HkS)".
   subst t.
+  iMod (db_update_token db with "token' token") as "(-> & token)".
   rewrite !later_equivI_1.
   case: HkS => [v0 Hv0].
   wp_bind (AList.find _ _).
@@ -146,8 +153,8 @@ iDestruct "disj" as "[#pub|car]".
   wp_bind (Sess.send _ _).
   iApply (wp_send_msg _ _ _ _
             (iMsg_dual (∃ v, MSG v {{ ⌜db !! k1 = Some v⌝ }};
-                          db_st skI skR cs db)%msg) _
-            (iProto_dual (db_st skI skR cs db))
+                          db_st skI skR cs (Some db))%msg) _
+            (iProto_dual (db_st skI skR cs (Some db)))
            with "[conn]").
   { iSplitL "conn".
     { iApply (connected_le with "conn"). iNext.
@@ -155,7 +162,7 @@ iDestruct "disj" as "[#pub|car]".
       rewrite iMsg_exist_eq iMsg_base_eq.
       iApply iProto_le_of_equiv. exact: iProto_dual_message. }
     iSplit => //.
-    iRight. iExists (db_st skI skR cs db).
+    iRight. iExists (db_st skI skR cs (Some db)).
     iSplit; last by auto.
     rewrite iMsg_exist_eq /=. iExists v0.
     rewrite iMsg_base_eq /=.
@@ -163,8 +170,8 @@ iDestruct "disj" as "[#pub|car]".
     iSplit; first by auto.
     by []. }
   iIntros "!> conn". wp_pures.
-  iApply ("post" $! true). iModIntro. iExists db.
-  by iFrame "rel vdb slot p_db conn".
+  iApply ("post" $! true). iModIntro. iExists (Some db), db.
+  by iFrame "rel vdb p_db conn"; eauto.
 Qed.
 
 Lemma wp_server_handle_create skI skR cs vdb :
@@ -176,36 +183,43 @@ Lemma wp_server_handle_create skI skR cs vdb :
 Proof.
 iIntros "#? #ctx".
 rewrite /server_handler /=.
-iIntros "!> %db %t %p !> %Φ (conn & rel & (#p_db & vdb & slot) & #p_t & disj) post".
+iIntros "!> %odb %db %t %p".
+iIntros "!> %Φ (conn & rel & (#p_db & vdb & token) & #p_t & disj) post".
 rewrite lookup_fmap db_arms_create /=.
 wp_pures. rewrite /Server.handle_create. wp_pures.
-iDestruct "disj" as "[#pub|car]".
--
-  wp_list_of_term t; wp_pures; last first.
-  { iApply ("post" $! true). iModIntro. iExists db. iFrame "rel vdb slot p_db".
+iPoseProof (or_sep1 with "token disj") as "[#pub|[token car]]".
+- wp_list_of_term t; wp_pures; last first.
+  { iApply ("post" $! true). iModIntro.
+    iExists (Some db), db. iFrame "rel vdb p_db".
+    iSplitL; eauto.
     by iApply (connected_repoint with "conn pub"). }
   wp_list_match => [k v ->|_]; wp_pures; last first.
-  { iApply ("post" $! true). iModIntro. iExists db. iFrame "rel vdb slot p_db".
+  { iApply ("post" $! true). iModIntro.
+    iExists (Some db), db. iFrame "rel vdb p_db".
+    iSplitL; eauto.
     by iApply (connected_repoint with "conn pub"). }
   rewrite public_of_list /=. iDestruct "p_t" as "(p_k & p_v & _)".
   wp_bind (AList.find _ _).
   iApply (AList.wp_find with "vdb").
   iIntros "!> vdb". rewrite lookup_fmap.
   case e: (db !! k) => [v0|] /=; wp_pures.
-  { iApply ("post" $! true). iModIntro. iExists db. iFrame "rel vdb slot p_db".
+  { iApply ("post" $! true). iModIntro.
+    iExists (Some db), db. iFrame "rel vdb p_db".
+    iSplitL; eauto.
     by iApply (connected_repoint with "conn pub"). }
   wp_bind (AList.insert _ _ _).
   iApply (AList.wp_insert with "vdb").
   iIntros "!> vdb". rewrite -fmap_insert. wp_pures.
-  iApply ("post" $! true). iModIntro. iExists (<[k := v]> db).
-  iFrame "rel vdb slot".
+  iApply ("post" $! true). iModIntro.
+  iExists (Some (<[k := v]> db)), (<[k := v]> db).
+  iFrame "rel vdb".
   iSplitL "conn"; first by iApply (connected_repoint with "conn pub").
+  iSplit; eauto.
   by iApply public_db_insert.
--
-  iDestruct "car" as (p1) "[car #HeqD]".
-  rewrite iMsg_exist_eq /=. iDestruct "car" as (k) "car".
+- iDestruct "car" as (p1) "[car #HeqD]".
+  rewrite iMsg_exist_eq /=. iDestruct "car" as (db0 k) "car".
   iDestruct "car" as (v) "car".
-  rewrite iMsg_base_eq /=. iDestruct "car" as "(%e_t & #Heq1 & %Hk)".
+  rewrite iMsg_base_eq /=. iDestruct "car" as "(%e_t & #Heq1 & token' & %Hk)".
   subst t.
   rewrite !later_equivI_1.
   rewrite public_of_list /=. iDestruct "p_t" as "(p_k & p_v & _)".
@@ -214,18 +228,20 @@ iDestruct "disj" as "[#pub|car]".
   wp_pures.
   wp_list_match => [k' v' e|ne]; last by case: (ne (eq_refl _)).
   case: e => <- <- {k' v'}. wp_pures.
+  iMod (db_update_token (<[k := v]> db) with "token' token")
+    as "(-> & token)".
   wp_bind (AList.find _ _).
   iApply (AList.wp_find with "vdb").
   iIntros "!> vdb". rewrite lookup_fmap Hk /=. wp_pures.
   wp_bind (AList.insert _ _ _).
   iApply (AList.wp_insert with "vdb").
   iIntros "!> vdb". rewrite -fmap_insert. wp_pures.
-  iApply ("post" $! true). iModIntro. iExists (<[k := v]> db).
-  iFrame "rel vdb slot".
+  iApply ("post" $! true). iModIntro. iExists (Some (<[k := v]> db)), _.
+  iFrame "rel vdb".
   iSplitL "conn".
   { iApply (connected_le with "conn"). iNext.
     iRewrite "HeqD". iRewrite -"Heq1". iApply iProto_le_refl. }
-  by iApply public_db_insert.
+  iFrame. by iApply public_db_insert.
 Qed.
 
 Lemma wp_server_handle_close skI skR cs vdb :
@@ -240,12 +256,12 @@ Lemma wp_server_handle_close skI skR cs vdb :
 Proof.
 iIntros "#? #ctx".
 rewrite /server_handler /=.
-iIntros "!> %db %t %p !> %Φ (conn & rel & (#p_db & vdb & slot) & #p_t & disj) post".
+iIntros "!> %odb %db %t %p".
+iIntros "!> %Φ (conn & rel & (#p_db & vdb & token) & #p_t & disj) post".
 rewrite lookup_fmap db_arms_close /=.
 wp_pures.
-iDestruct "disj" as "[#pub|car]".
--
-  iDestruct (connected_public_key_or' _ _ _ _ _ False%I
+iDestruct (or_sep1 with "token disj") as "[#pub|[token car]]".
+- iDestruct (connected_public_key_or' _ _ _ _ _ False%I
               with "conn rel []") as "(conn & rel & >comp)"; first by iLeft.
   iDestruct "comp" as "[#comp|[]]".
   iPoseProof (connected_failure' with "conn comp") as "#fail".
@@ -259,53 +275,37 @@ iDestruct "disj" as "[#pub|car]".
   wp_pures.
   iApply ("post" $! false). iModIntro. iExists db.
   iFrame "vdb p_db". by iLeft.
--
-  iDestruct "car" as (p1) "[car #HeqD]".
-  rewrite iMsg_base_eq /=. iDestruct "car" as "(%e_t & #Heq1 & client_busy)".
+- iDestruct "car" as (p1) "[car #HeqD]".
+  rewrite iMsg_base_eq /=.
+  rewrite iMsg_exist_eq /=.
+  iDestruct "car" as "(%db0 & %e_t & #Heq1 & token')".
   rewrite !later_equivI_1.
-  iDestruct "slot" as "[#comp|server_busy]".
-  +
-    iPoseProof (connected_failure' with "conn comp") as "#fail".
-    iPoseProof (compromised_public with "comp") as "#pub".
-    wp_bind (Sess.send _ _).
-    iApply (wp_send _ _ _ _ (TInt 0) END with "[conn]").
-    { iSplit; last by rewrite public_TInt.
-      by iApply (connected_repoint with "conn pub"). }
-    iIntros "!> conn". wp_pures.
-    iDestruct "conn" as "[gc _]".
-    wp_apply (GenConn.wp_free with "gc"). iIntros "_".
-    wp_pures.
-    iApply ("post" $! false). iModIntro. iExists db.
-    iFrame "vdb p_db". by iLeft.
-  +
-    iMod (db_close_resp skI skR db with "server_busy client_busy")
-      as "[client_ready server_ready]".
-    iMod (cryptis.examples.iso_dh.proofs.base.release with "rel") as "#relR".
-    wp_bind (Sess.send _ _).
-    iApply (wp_send_msg _ _ _ _
-              (iMsg_dual (MSG (TInt 0)
-                 {{ db_client_ready skI skR db ∗
-                    released (si_resp_share cs) }}; END)%msg) _
-              (iProto_dual END)
-             with "[conn client_ready]").
-    { iSplitL "conn".
-      { iApply (connected_le with "conn"). iNext.
-        iRewrite "HeqD". iRewrite -"Heq1".
-        rewrite iMsg_base_eq.
-        iApply iProto_le_of_equiv. exact: iProto_dual_message. }
-      iSplit; first by rewrite public_TInt.
-      iRight. iExists END.
-      iSplit; last by auto.
-      rewrite iMsg_base_eq /=.
-      iSplit; first done.
-      iSplit; first by auto.
-      by iFrame "client_ready relR". }
-    iIntros "!> conn". wp_pures.
-    iDestruct "conn" as "[gc _]".
-    wp_apply (GenConn.wp_free with "gc"). iIntros "_".
-    wp_pures.
-    iApply ("post" $! false). iModIntro. iExists db.
-    iFrame "vdb p_db". by iRight.
+  iMod (db_update_token db with "token' token") as "(-> & _ & main & copy)".
+  iMod (cryptis.examples.iso_dh.proofs.base.release with "rel") as "#relR".
+  wp_bind (Sess.send _ _).
+  iApply (wp_send_msg _ _ _ _
+            (iMsg_dual (MSG (TInt 0)
+               {{ db_main' skI skR db ∗
+                  released (si_resp_share cs) }}; END)%msg) _
+            (iProto_dual END)
+           with "[conn main]").
+  { iSplitL "conn".
+    { iApply (connected_le with "conn"). iNext.
+      iRewrite "HeqD". iRewrite -"Heq1".
+      rewrite iMsg_base_eq.
+      iApply iProto_le_of_equiv. exact: iProto_dual_message. }
+    iSplit; first by rewrite public_TInt.
+    iRight. iExists END.
+    iSplit; last by auto.
+    rewrite iMsg_base_eq /=.
+    iSplit; first done.
+    iSplit; first by auto. by iFrame. }
+  iIntros "!> conn". wp_pures.
+  iDestruct "conn" as "[gc _]".
+  wp_apply (GenConn.wp_free with "gc"). iIntros "_".
+  wp_pures.
+  iApply ("post" $! false). iModIntro. iExists db.
+  iFrame "vdb p_db". by iRight.
 Qed.
 
 Lemma wp_handle' N f φ :
@@ -326,70 +326,24 @@ Lemma wp_server_conn_handler skI skR cs vdb vlock γlock db :
   cryptis_ctx -∗
   store_ctx -∗
   is_lock γlock vlock (server_db_disconnected skI skR vdb) -∗
-  {{{ connected skI skR Resp cs (iProto_dual (db_st0 skI skR cs)) ∗
+  {{{ connected skI skR Resp cs (iProto_dual (db_st skI skR cs None)) ∗
       release_token (si_resp_share cs) ∗
-      (public (si_key cs) ∨ db_server_ready skI skR db) ∗
+      (public (si_key cs) ∨ db_copy' skI skR db) ∗
       public_db db ∗
       AList.is_alist vdb (repr <$> db) ∗
       locked γlock }}}
     Server.conn_handler (repr cs) vdb vlock
   {{{ RET #(); True }}}.
 Proof.
-iIntros "#? #ctx #lock !> %Φ (conn & rel & ready & #p_db & vdb & locked) post".
+iIntros "#? #ctx #lock !> %Φ (conn & rel & copy & #p_db & vdb & locked) post".
 iPoseProof (wp_server_handle_store skI skR cs vdb with "[//] [//]") as "#Hst".
 iPoseProof (wp_server_handle_load skI skR cs vdb with "[//] [//]") as "#Hld".
 iPoseProof (wp_server_handle_create skI skR cs vdb with "[//] [//]") as "#Hcr".
 iPoseProof (wp_server_handle_close skI skR cs vdb with "[//] [//]") as "#Hcl".
 wp_lam. wp_pures.
-
-wp_bind (Sess.recv _).
-iApply (wp_recv _ _ _ _
-          (iMsg_tag (iMsg_dual <$>
-             ({[dbN.@"connect" :=
-                  (∃ db', MSG (TInt 0)
-                     {{ rep_update skI skR dbN ∅ db' db' }};
-                   db_st skI skR cs db')%msg]}
-              : gmap namespace (iMsg Σ term))))
-         with "[conn]").
-{ iApply (connected_le with "conn"). iNext.
-  iApply iProto_le_of_equiv.
-  by rewrite /db_st0 iProto_dual_tag /iProto_tag. }
-iIntros "!> %t %p (#p_t & conn & disj)".
-iDestruct (connected_public_key_or' with "conn rel disj")
-  as "(conn & rel & >disj)".
 iAssert (|={⊤}=> server_db_connected skI skR cs vdb)%I
-  with "[conn rel ready vdb disj]" as ">sdc".
-{ iDestruct "disj" as "[#comp|car]".
-  { iModIntro. iExists db.
-    iSplitL "conn".
-    { by iApply (connected_compromised with "conn comp"). }
-    iFrame "rel vdb p_db". by iLeft. }
-  rewrite iMsg_tag_eq.
-  iDestruct "car" as (N t' m) "[%em car]".
-  case: em => em ->.
-  move: em. rewrite lookup_fmap.
-  case em0: ({[_ := _]} !! N) => [m0|] //= => - [<-] {m}.
-  case/lookup_singleton_Some: em0 => <- <- {N m0}.
-  iDestruct "car" as (p1) "[car #HeqD]".
-  rewrite iMsg_exist_eq /=. iDestruct "car" as (db') "car".
-  rewrite iMsg_base_eq /=. iDestruct "car" as "(_ & #Heq1 & upd)".
-  rewrite !later_equivI_1.
-  iDestruct "ready" as "[#pub|ready]".
-  { iDestruct (connected_public_key_or' _ _ _ _ _ False%I
-                with "conn rel []") as "(conn & rel & >comp)";
-      first by iLeft.
-    iDestruct "comp" as "[#comp|[]]".
-    iModIntro. iExists db.
-    iSplitL "conn".
-    { by iApply (connected_compromised with "conn comp"). }
-    iFrame "rel vdb p_db". by iLeft. }
-  iMod (db_connect_resp with "ready upd") as "(%e & busy)".
-  subst db'.
-  iModIntro. iExists db.
-  iSplitL "conn".
-  { iApply (connected_le with "conn"). iNext.
-    iRewrite "HeqD". iRewrite -"Heq1". iApply iProto_le_refl. }
-  iFrame "rel vdb p_db". by iRight. }
+  with "[conn rel copy vdb]" as ">sdc".
+{ iModIntro. iExists None, db. iFrame; eauto. }
 wp_pures.
 
 wp_bind (Sess.handle _ _). iApply wp_handle'.
@@ -403,7 +357,7 @@ iIntros "%h_st %e_st". subst h_st. wp_list.
 wp_pures.
 
 iLöb as "IH".
-iDestruct "sdc" as (db') "(conn & rel & sdc')".
+iDestruct "sdc" as (odb db') "(conn & rel & sdc')".
 pose (handlers :=
   [Handler (dbN.@"store")
      (λ: "req", Server.handle_store vdb "req";; #true)%V;
@@ -435,10 +389,10 @@ iApply (wp_wand _ _ _ φ with "[conn rel sdc']"); last first.
     + wp_apply (release_spec with "[$lock $locked $Hb]").
       iIntros "_". by iApply "post". }
 iApply (@wp_select' skI skR Resp cs
-          (iMsg_dual <$> db_arms skI skR cs (db_st skI skR cs) db')
+          (iMsg_dual <$> db_arms skI skR cs (db_st skI skR cs) odb)
           handlers
           (release_token (si_resp_share cs) ∗
-           server_db_connected' skI skR cs vdb db')%I
+           server_db_connected' skI skR cs vdb odb db')%I
           φ
          with "[conn] [rel sdc'] [] []").
 - rewrite dom_fmap_L db_arms_dom /=. set_solver.
@@ -449,23 +403,23 @@ iApply (@wp_select' skI skR Resp cs
   rewrite /select_vc /=.
   iSplit.
   { iIntros "%tm %pm conn #p_tm disj".
-    iApply ("Hst" $! db' tm pm with "[$conn $rel $sdc' $p_tm $disj]").
+    iApply ("Hst" $! odb db' tm pm with "[$conn $rel $sdc' $p_tm $disj]").
     iIntros "!> %b Hb". iRight. iExists b. by iFrame. }
   iSplit.
   { iIntros "%tm %pm conn #p_tm disj".
-    iApply ("Hld" $! db' tm pm with "[$conn $rel $sdc' $p_tm $disj]").
+    iApply ("Hld" $! odb db' tm pm with "[$conn $rel $sdc' $p_tm $disj]").
     iIntros "!> %b Hb". iRight. iExists b. by iFrame. }
   iSplit.
   { iIntros "%tm %pm conn #p_tm disj".
-    iApply ("Hcr" $! db' tm pm with "[$conn $rel $sdc' $p_tm $disj]").
+    iApply ("Hcr" $! odb db' tm pm with "[$conn $rel $sdc' $p_tm $disj]").
     iIntros "!> %b Hb". iRight. iExists b. by iFrame. }
   iSplit; last done.
   iIntros "%tm %pm conn #p_tm disj".
-  iApply ("Hcl" $! db' tm pm with "[$conn $rel $sdc' $p_tm $disj]").
+  iApply ("Hcl" $! odb db' tm pm with "[$conn $rel $sdc' $p_tm $disj]").
   iIntros "!> %b Hb". iRight. iExists b. by iFrame.
 - iIntros "%pm conn #pub [rel sdc']".
   iLeft. iSplit => //.
-  iExists db'. iFrame "rel sdc'".
+  iExists odb, db'. iFrame "rel sdc'".
   by iApply (connected_repoint with "conn pub").
 Qed.
 
@@ -551,6 +505,7 @@ case accounts_skI: (accounts !! Spec.pkey skI) => [scs|]; wp_pures.
     iExists _. iSplit => //.
 Qed.
 
+(* TODO: This should follow from Sess.wp_confirm *)
 Lemma wp_confirm' (P : iProp) c skI skR ga :
   channel c -∗
   cryptis_ctx -∗
@@ -559,7 +514,7 @@ Lemma wp_confirm' (P : iProp) c skI skR ga :
       (GenConn.failure skI skR ∨ P) }}}
     Sess.confirm c skR (Tag dbN) (ga, Spec.pkey skI)%V
   {{{ cs, RET (repr cs);
-      connected skI skR Resp cs (iProto_dual (db_st0 skI skR cs)) ∗
+      connected skI skR Resp cs (iProto_dual (db_st skI skR cs None)) ∗
       release_token (si_resp_share cs) ∗
       (public (si_key cs) ∨ P) }}}.
 Proof.
@@ -570,7 +525,7 @@ wp_apply (GenConn.wp_confirm P with "[] [$P]").
 - eauto.
 - do 3!iSplit => //.
   iIntros "!> %b tok".
-  iMod (iProto_init (db_st0 skI skR _)) as (γl γr) "(pctx & ownI & ownR)".
+  iMod (iProto_init (db_st skI skR _ None)) as (γl γr) "(pctx & ownI & ownR)".
   iMod (term_meta_set (sessN.@"names") (γl, γr) with "tok") as "#meta".
   { solve_ndisj. }
   iModIntro. iSplitL "ownI".
@@ -602,7 +557,7 @@ iDestruct "dis" as "(%db & #p_db & vdb & ready)".
 iAssert (minted (ss_key ss)) as "#?".
 { by iDestruct "server" as "(% & % & ? & _)". }
 wp_pures.
-wp_apply (wp_confirm' (db_server_ready skA (ss_key ss) db)
+wp_apply (wp_confirm' (db_copy' skA (ss_key ss) db)
            with "chan_c cctx ctx [ready]").
 { do 3?(iSplit; [done|]). iExact "ready". }
 iIntros "%cs (conn & rel & ready)". wp_pures.
